src/PredMsg.v
@@ -1,0 +1,214 @@
+Require Import Bool List String Peano_dec.
+Require Import Common FMap.
+Require Import Syntax Semantics.
+
+Set Implicit Arguments.
+
+Inductive RqRs := Rq | Rs.
+
+Definition OPred :=
+  Value (* input *) -> OrdOState -> Value (* output *) -> Prop.
+
+Definition Pred :=
+  Value (* input *) -> ObjectStates OrdOState -> Value (* output *) -> Prop.
+
+Record OTrs :=
+  { otrs_rqval: Value;
+    otrs_rqpred: Pred;
+    otrs_opred: OPred;
+    otrs_rsbf: list Value -> OrdOState -> Value }.
+
+Inductive PMsg : RqRs -> Type :=
+| PMsgIntro: forall (mid: MsgId) (rr: RqRs) (val: Value) (pred: Pred), PMsg rr.
+
+Definition midOfPMsg {rr} (pmsg: PMsg rr): MsgId :=
+  match pmsg with
+  | PMsgIntro mid _ _ _ => mid
+  end.
+
+Definition valOfPMsg {rr} (pmsg: PMsg rr): Value :=
+  match pmsg with
+  | PMsgIntro _ _ val _ => val
+  end.
+
+Definition predOfPMsg {rr} (pmsg: PMsg rr): Pred :=
+  match pmsg with
+  | PMsgIntro _ _ _ pred => pred
+  end.
+
+Global Instance PMsg_HasMsg (rr: RqRs): HasMsg (PMsg rr) :=
+  {| getMsg := fun pmsg =>
+                 match pmsg with
+                 | PMsgIntro mid rr val pred => buildMsg mid val
+                 end |}.
+
+Global Instance PMsg_sigT_HasMsg : HasMsg { rr : RqRs & PMsg rr } :=
+  {| getMsg := fun pmsg =>
+                 match projT2 pmsg with
+                 | PMsgIntro mid rr val pred => buildMsg mid val
+                 end |}.
+
+Section PLabel.
+
+  Inductive PLabel :=
+  | PlblEmpty: PLabel
+  | PlblIn (min: PMsg Rq): PLabel
+  | PlblImm (min: PMsg Rq) (mout: PMsg Rs): PLabel
+  | PlblRqFwd (min: PMsg Rq) (mfwds: list (PMsg Rq)): PLabel
+  | PlblRsBack (mins: list (PMsg Rs)) (mback: PMsg Rs): PLabel.
+
+  Definition pToLabel (l: PLabel): Label :=
+    match l with
+    | PlblEmpty => LblOuts nil
+    | PlblIn min => LblIn (getMsg min)
+    | PlblImm min mout => LblOuts (getMsg mout :: nil)
+    | PlblRqFwd min mfwds => LblOuts (map getMsg mfwds)
+    | PlblRsBack mins mback => LblOuts (getMsg mback :: nil)
+    end.
+
+  Global Instance PLabel_HasLabel: HasLabel PLabel :=
+    { getLabel := pToLabel }.
+
+End PLabel.
+
+Record PObject :=
+  { pobj_idx: nat;
+    pobj_state_init: OrdOState
+  }.
+
+Global Instance PObject_IsObject : IsObject OrdOState PObject :=
+  {| getIndex := pobj_idx;
+     getOStateInit := pobj_state_init |}.
+
+Definition Topo := list MsgAddr.
+
+Record PSystem :=
+  { psys_topo: Topo;
+    psys_obs: list PObject }.
+
+Global Instance PSystem_HasObjects : HasObjects PSystem :=
+  {| getObjects := psys_obs |}.
+
+Record PState :=
+  { pst_oss: ObjectStates OrdOState;
+    pst_otrs: M.t OTrs;
+    pst_msgs: MessagePool { rr: RqRs & PMsg rr }
+  }.
+
+Definition getPStateInit (psys: PSystem): PState :=
+  {| pst_oss := getObjectStatesInit (psys_obs psys);
+     pst_otrs := [];
+     pst_msgs := nil |}.
+
+Global Instance PState_HasInit: HasInit PSystem PState :=
+  { getStateInit := getPStateInit }.
+
+(* Definition PHistory := list PLabel. *)
+
+(* Inductive step_pred: PSystem -> PState -> PHistory -> PState -> Prop := *)
+(* | SpDone: forall psys st, step_pred psys st nil st *)
+(* | SpSlt: forall psys st1 st2 hst, *)
+(*     step_pred psys st1 hst st2 -> *)
+(*     step_pred psys st1 (PlblEmpty :: hst) st2 *)
+
+(* | SpIn: *)
+(*     forall psys mid val pred oss otrs msgs phst pst, *)
+(*       isExternal psys (mid_from mid) = true -> *)
+(*       isInternal psys (mid_to mid) = true -> *)
+
+(*       step_pred psys *)
+(*                 {| pst_oss := oss; *)
+(*                    pst_otrs := otrs; *)
+(*                    pst_msgs := enqMP (existT _ _ (PMsgIntro mid Rq val pred)) msgs *)
+(*                 |} *)
+(*                 phst pst -> *)
+
+(*       step_pred psys *)
+(*                 {| pst_oss := oss; pst_otrs := otrs; pst_msgs := msgs |} *)
+(*                 (PlblIn (PMsgIntro mid Rq val pred) :: phst) *)
+(*                 pst. *)
+
+Inductive step_pred (psys: PSystem): PState -> PLabel -> PState -> Prop :=
+| SpSlt: forall st, step_pred psys st PlblEmpty st
+
+| SpIn:
+    forall mid val pred oss otrs msgs,
+      isExternal psys (mid_from mid) = true ->
+      isInternal psys (mid_to mid) = true ->
+      step_pred psys
+                {| pst_oss := oss; pst_otrs := otrs; pst_msgs := msgs |}
+                (PlblIn (PMsgIntro mid Rq val pred))
+                {| pst_oss := oss;
+                   pst_otrs := otrs;
+                   pst_msgs := enqMP (existT _ _ (PMsgIntro mid Rq val pred)) msgs
+                |}
+
+| SpImm:
+    forall mid rq rs rqVal rsVal pred oidx nos oss otrs msgs,
+      rq = PMsgIntro mid Rq rqVal pred ->
+      rs = PMsgIntro mid Rs rsVal pred ->
+
+      FirstMP msgs (existT _ _ rq) ->
+      ValidMsgsIn oidx (rq :: nil) ->
+      ValidMsgOuts oidx (rs :: nil) ->
+      pred rqVal (oss +[oidx <- nos]) rsVal ->
+
+      step_pred psys
+                {| pst_oss := oss; pst_otrs := otrs; pst_msgs := msgs |}
+                (PlblImm rq rs)
+                {| pst_oss := oss +[ oidx <- nos ];
+                   pst_otrs := otrs;
+                   pst_msgs := distributeMsgs
+                                 (intOuts psys (existT _ _ rs :: nil))
+                                 (removeMP (existT _ _ rq) msgs) |}
+
+| SpRqFwd:
+    forall oidx rq fwds oss otrs opred rsbf msgs,
+      FirstMP msgs (existT _ _ rq) ->
+      ValidMsgsIn oidx (rq :: nil) ->
+      ValidMsgOuts oidx fwds ->
+      Forall (fun pmsg =>
+                isInternal psys (mid_to (msg_id (getMsg pmsg))) = true) fwds ->
+      
+      step_pred psys
+                {| pst_oss := oss; pst_otrs := otrs; pst_msgs := msgs |}
+                (PlblRqFwd rq fwds)
+                {| pst_oss := oss;
+                   pst_otrs := otrs +[ oidx <- {| otrs_rqval := valOfPMsg rq;
+                                                  otrs_rqpred := predOfPMsg rq;
+                                                  otrs_opred := opred;
+                                                  otrs_rsbf := rsbf |} ];
+                   pst_msgs := distributeMsgs
+                                 (map (fun pmsg => existT _ _ pmsg) fwds)
+                                 (removeMP (existT _ _ rq) msgs) |}
+
+| SpRsBack:
+    forall oidx rss rsb otrs ootrs oss msgs,
+      Forall (FirstMP msgs) (map (existT _ _) rss) ->
+      ValidMsgsIn oidx rss ->
+      ValidMsgOuts oidx (rsb :: nil) ->
+      Forall (fun pmsg =>
+                isInternal psys (mid_from (msg_id (getMsg pmsg))) = true) rss ->
+
+      otrs@[oidx] = Some ootrs ->
+      
+      (* predOfPMsg rsb (otrs_rqval rqval) (oss +[oidx <- nos]) (valOfPMsg rsb) *)
+
+      step_pred psys
+                {| pst_oss := oss; pst_otrs := otrs; pst_msgs := msgs |}
+                (PlblRsBack rss rsb)
+                {| pst_oss := oss;
+                   pst_otrs := M.remove oidx otrs;
+                   pst_msgs := distributeMsgs
+                                 (intOuts psys (existT _ _ rsb :: nil))
+                                 (removeMsgs (map (existT _ _) rss) msgs) |}.
+
+(** What we want, informally:
+ * - [step_det] with particular rules -> [step_pred]
+ * - [step_det] with particular rules -> [Transactional] history ->
+ *   postconditions in [step_pred] are preserved.
+ *
+ * - Do we need to specify preconditions in [step_pred]? I think no, because
+ *   those are only about "sate interleavings", i.e., serializability.
+*)
+
