src/Serial.v
@@ -4,7 +4,7 @@ Require Import Common ListSupport FMap Syntax Semantics StepDet.
 (** [Atomic] and [Transactional] histories *)
 
 Section PerSystem.
-  Variable sys: System.
+  Variable sys: System OrdOState.
 
   (* A history is [Atomic] if it satisfies following conditions:
    * 1) The history can be either an incomplete or a complete transaction.
@@ -13,7 +13,7 @@ Section PerSystem.
    *    and all [hdl]s have the same [tinfo_tid]. It means that the history is
    *    for a single transaction.
    *)
-  Inductive Atomic: TrsId -> Msg -> History -> MessagePool TMsg -> Prop :=
+  Inductive Atomic: TrsId -> Msg -> THistory -> MessagePool TMsg -> Prop :=
   | AtomicStart:
       forall ts rqr rq houts,
         isExternal sys (mid_from (msg_id rq)) = true ->
@@ -28,9 +28,9 @@ Section PerSystem.
         Atomic ts rq (IlblOuts (Some rule) msgs houts :: hst)
                (distributeMsgs houts (removeMsgs msgs mouts)).
 
-  Inductive Transactional: History -> Prop :=
+  Inductive Transactional: THistory -> Prop :=
   | TrsSlt:
-      Transactional (emptyILabel :: nil)
+      Transactional (emptyRLabel :: nil)
   | TrsIn:
       forall msg tin,
         tin = IlblIn msg ->
@@ -40,8 +40,8 @@ Section PerSystem.
         Atomic ts rq hst mouts ->
         Transactional hst.
 
-  Definition Sequential (hst: History) :=
-    exists trss: list History,
+  Definition Sequential (hst: THistory) :=
+    exists trss: list THistory,
       Forall Transactional trss /\
       hst = concat trss.
 
@@ -58,25 +58,25 @@ Definition trsMessages (trsInfo: TInfo) (mp: MessagePool TMsg) : list TMsg :=
 
 (** Serializability *)
 
-Definition trsSteps (sys: System) (st1: TState) (hst: History) (st2: TState) :=
+Definition trsSteps (sys: System OrdOState) (st1: TState) (hst: THistory) (st2: TState) :=
   steps_det sys st1 hst st2 /\
   Transactional sys hst.
 
-Definition seqSteps (sys: System) (st1: TState) (hst: History) (st2: TState) :=
+Definition seqSteps (sys: System OrdOState) (st1: TState) (hst: THistory) (st2: TState) :=
   steps_det sys st1 hst st2 /\
   Sequential sys hst.
 
-Definition Equivalent (sys: System)
+Definition Equivalent (sys: System OrdOState)
            {LabelT} `{HasLabel LabelT} (ll1 ll2: list LabelT) :=
   behaviorOf sys ll1 = behaviorOf sys ll2.
 
-Definition Serializable (sys: System) (ll: History) :=
+Definition Serializable (sys: System OrdOState) (ll: THistory) :=
   exists sll sst,
     (* 1) legal and sequential *) seqSteps sys (getStateInit sys) sll sst /\
     (* 3) equivalent *) Equivalent sys ll sll.
 
 (* A system is serializable when all possible behaviors are [Serializable]. *)
-Definition SerializableSys (sys: System) :=
+Definition SerializableSys (sys: System OrdOState) :=
   forall ll st,
     steps_det sys (getStateInit sys) ll st ->
     Serializable sys ll.
